Port exBs examples from test suite to Coq

Coq/src/Example.v
@@ -2,16 +2,346 @@ Require Import Thesis.Handler.
 Require Import Thesis.Effect.
 Require Import Thesis.Free.
 Require Import Thesis.Base.
+Require Import Lists.List.
+
+Import List.ListNotations.
 
 Set Implicit Arguments.
 
-Example p1 : Prog (nat * nat) := Share Coin >>= fun x => duplicate x.
-Lemma l1 : handle e1 = ((0, 0) :: (1, 1) :: Datatypes.nil)%list.
+Definition coin := Coin__Bool.
+Definition share := Share.
+Definition const := fun A (x _ : A) => x.
+Definition cons := Effect.cons.
 
-Example e2 : Prog nat := Share Coin >>= fun x => addM x x.
-Lemma l2 : handle e2 = (0 :: 2 :: Datatypes.nil)%list.
+Example example1 : Prog bool := coin.
+Example res_example1 := [true; false].
 
-Example e3 : Prog bool := orM (pure true) Fail.
-Lemma l3 : handle e3 = (true :: Datatypes.nil)%list.
+Example example2 : Prog bool := coin ? coin.
+Example res_example2 := [true; false; true; false].
 
-Definition ls := (l1 :: l2 :: l3 :: Datatypes.nil)%list.
+Example example3 : Prog bool :=  share coin >>= fun fx => fx ? fx.
+Example res_example3 := res_example2.
+
+Example exOr0 : Prog bool := orM coin (pure false).
+Example res_exOr0 := [true; false].
+
+Example exOr1 : Prog bool := orM coin coin.
+Example res_exOr1 := [true; true; false].
+
+Example exOr2 : Prog bool := share coin >>= fun fx => orM fx fx.
+Example res_exOr2 := [true; false].
+
+Example exOr2a : Prog bool :=
+  share coin >>= fun fx => orM (pure false) (orM fx fx).
+Example res_exOr2a := [true; false].
+
+Example exOr2b : Prog bool :=
+  share coin >>= fun fx => orM (pure true) (orM fx fx).
+Example res_exOr2b := [true].
+
+Example exOr3 : Prog bool := orM (coin ? coin) (pure true).
+Example res_exOr3 := [true; true; true; true].
+
+Example exOr3a : Prog bool := orM (coin ? coin) coin.
+Example res_exOr3a := [true; true; false; true; true; false].
+
+Example exOr3b : Prog bool := orM coin (coin ? coin).
+Example res_exOr3b := [true; true; false; true; false].
+
+Example exOr3c : Prog bool := orM (coin ? coin) (coin ? coin).
+Example res_exOr3c := [true; true; false; true; false; true; true; false; true; false].
+
+(* here we share, even though nothing is shared *)
+Example exOr4 : Prog bool := share coin >>= fun fx => orM fx coin.
+Example res_exOr4 := [true; true; false].
+
+Example exOrShare : Prog bool := share coin >>= fun fx => orM coin fx.
+Example res_exOrShare := [true; true; false].
+
+Example exOr6 : Prog bool := share coin >>= fun fx => orM fx (orM fx coin).
+Example res_exOr6 := [true; true; false].
+
+Example exOr7 : Prog bool := share coin >>= fun fx => orM coin (orM fx fx).
+Example res_exOr7 := [true; true; false].
+
+Example exOr7a : Prog bool := share coin >>= fun fx => orM (pure true) (orM fx fx).
+Example res_exOr7a := [true].
+
+Example exOr7b : Prog bool := share coin >>= fun fx => orM (pure false) (orM fx fx).
+Example res_exOr7b := [true; false].
+
+Example exShareConst : Prog bool := share coin >>= fun fx => const fx fx.
+Example res_exShareConst := [true; false].
+
+Example exShareConstOrR : Prog bool := share coin >>= fun fx => orM fx (const fx fx).
+Example res_exShareConstOrR := [true; false].
+
+Example exShareConstOrL : Prog bool := share coin >>= fun fx => orM (const fx fx) fx.
+Example res_exShareConstOrL := [true; false].
+
+Example exShareConstOrR2 : Prog bool := share coin >>= fun fx => orM (pure true) (const fx fx).
+Example res_exShareConstOrR2 := [true].
+
+Example exFailed : Prog bool := share Fail >>= fun fx => const (pure true) fx.
+Example res_exFailed := [true].
+
+Example exHead : Prog bool := headM (cons coin Fail).
+Example res_exHead := [true; false].
+
+Example exOrShareShare : Prog bool :=
+  share coin >>=
+        fun fx =>
+          share coin >>=
+                fun fy =>
+                  orM fx (orM fy (orM fx fy)).
+Example res_exOrShareShare := [true; true; false].
+
+Example exOrShareNested : Prog bool :=
+  share coin >>= fun fx =>
+                   orM fx (share coin >>= fun fy =>
+                                            orM fy (orM fx fy)).
+Example res_exOrShareNested := [true; true; false].
+
+Example exShareNestedChoiceOr : Prog bool :=
+  share ((pure true ? pure false) ? (pure true ? pure false)) >>=
+        fun fx => orM fx fx.
+Example res_exShareNestedChoiceOr := [true; false; true; false].
+
+Example exShareIgnoreShare : Prog bool :=
+  share coin >>= fun fx => const (pure true) (share fx >>= fun fy => orM fy fy).
+Example res_exShareIgnoreShare := [true].
+
+Example exRepeatedShare : Prog bool :=
+  share coin >>= fun fx => share fx >>= fun fy => orM fy fy.
+Example res_exRepeatedShare := [true; false].
+
+Definition exBs := [(example1, res_example1);
+                      (example2, res_example2);
+                      (example3, res_example3);
+                      (exOr0, res_exOr0);
+                      (exOr1, res_exOr1);
+                      (exOr2, res_exOr2);
+                      (exOr2a, res_exOr2a);
+                      (exOr2b, res_exOr2b);
+                      (exOr3, res_exOr3);
+                      (exOr3a, res_exOr3a);
+                      (exOr3b, res_exOr3b);
+                      (exOr3c, res_exOr3c);
+                      (exOr4, res_exOr4);
+                      (exOrShare, res_exOrShare);
+                      (exOr6, res_exOr6);
+                      (exOr7, res_exOr7);
+                      (exOr7a, res_exOr7a);
+                      (exOr7b, res_exOr7b);
+                      (exShareConst, res_exShareConst);
+                      (exShareConstOrR, res_exShareConstOrR);
+                      (exShareConstOrL, res_exShareConstOrL);
+                      (exShareConstOrR2, res_exShareConstOrR2);
+                      (exFailed, res_exFailed);
+                      (exHead, res_exHead);
+                      (exOrShareShare, res_exOrShareShare);
+                      (exOrShareNested, res_exOrShareNested);
+                      (exShareNestedChoiceOr, res_exShareNestedChoiceOr);
+                      (exShareIgnoreShare, res_exShareIgnoreShare);
+                      (exRepeatedShare, res_exRepeatedShare)].
+                      
+Lemma tests__exBs : Forall (fun '(p,r) => handle p = r) exBs.
+Proof. repeat econstructor. Qed.
+(*
+exOrShareNestedList :: (Sharing m, MonadPlus m) => m (List m Bool)
+exOrShareNestedList = share coin >>= \fx ->
+                  cons fx (share coin >>= \fy ->
+                              cons fy (cons fx (cons fy nil)))
+
+recList :: (Sharing m, MonadPlus m) => m (List m Bool) -> m (List m Bool)
+recList fxs = fxs >>= \xfps -> case xfps of
+                                    Nil -> nil
+                                    Cons fy fys -> share fys >>= \fys' -> cons fy (fys' `mplus` recList fys')
+
+exRecList :: (Sharing m, MonadPlus m) => m (Pair m (List m Bool))
+exRecList = share (recList (cons (return True) (cons (return False) nil))) >>= \fx -> pairM fx fx
+
+exRecListNested :: (Sharing m, MonadPlus m) => m (List m (List m Bool))
+exRecListNested = share (recList (cons (return True) (cons (return False) nil)))
+  >>= \fx -> cons fx (share (recList (cons (return True) (cons (return False) nil)))
+                      >>= \fz -> cons fz (cons fx (cons fz nil)))
+exSkipIds :: (Sharing m, MonadPlus m) => m Bool
+exSkipIds = share coin >>= \fx -> const coin (const fx fx)
+exLoop :: Sharing m => m Bool
+exLoop = let loop :: m ()
+             loop = loop in share loop >>= \fx -> const (return True) (const fx fx)
+exLoop2 :: Sharing m => m Bool
+exLoop2 = let loop :: m ()
+              loop = loop in share loop >>= \fx -> const coin (const fx fx)
+
+exDup :: (Sharing m, MonadPlus m) => m (Pair m Bool)
+exDup = dup coin
+exDupShare :: (Sharing m, MonadPlus m) => m (Pair m Bool)
+exDupShare = share coin >>= dup
+exDupShare2 :: (Sharing m, MonadPlus m) => m (Pair m Bool)
+exDupShare2 = dupShare coin
+exDupFailed :: (Sharing m, MonadPlus m) => m (Pair m Bool)
+exDupFailed = share (mzero :: MonadPlus m => m Bool) >>= \x -> dup (const (return True) x)
+exDupFirst :: MonadPlus m => m (Pair m Bool)
+exDupFirst = dup (first (pairM coin mzero))
+exDupShareFirst :: (Sharing m, MonadPlus m) => m (Pair m Bool)
+exDupShareFirst = dupShare (first (pairM coin mzero))
+
+exDupl :: MonadPlus m => m (List m Bool)
+exDupl = dupl (headM (cons coin (mzero :: MonadPlus m => m (List m Bool))))
+exDupl2 :: MonadPlus m => m (List m Bool)
+exDupl2 = cons (headM (cons coin (mzero :: MonadPlus m => m (List m Bool))))
+               (cons (headM (cons coin (mzero :: MonadPlus m => m (List m Bool))))
+                     nil)
+exDuplShare :: (Sharing m, MonadPlus m) => m (List m Bool)
+exDuplShare = duplShare (headM (cons coin (mzero :: MonadPlus m => m (List m Bool))))
+
+exShareNestedChoice :: (Sharing m, MonadPlus m) => m (Pair m Bool)
+exShareNestedChoice =
+  share (mplus (mplus (return True) (return False)) (mplus (return True) (return False))) >>=
+    \fx -> pairM fx fx
+
+
+exShareNestedChoice2 :: (Sharing m, MonadPlus m) => m (List m Bool)
+exShareNestedChoice2 =
+  share (mplus (return True) (mplus (return False) (return True))) >>=
+    \fx -> share (mplus (return True) (return False)) >>= \fy -> cons fx (cons fy (cons fx (cons fy nil)))
+
+
+exShareSingleton :: (Sharing m, MonadPlus m) => m (Pair m (List m Bool))
+exShareSingleton =
+  share (cons (return True `mplus` return False) nil) >>=
+    \fx -> pairM fx fx
+
+exShareInShare :: (Sharing m, MonadPlus m) => m (Pair m Bool)
+exShareInShare = share (share coin >>= \fx -> orM fx fx) >>= \fy -> pairM fy fy
+
+exShareListInShare :: (Sharing m, MonadPlus m) => m (Pair m (List m Bool))
+exShareListInShare =
+  share (share (cons coin (cons coin nil)) >>=
+          \fx -> appM fx fx) >>= \fy -> pairM fy fy
+
+exSharePutPos :: (Sharing m, MonadPlus m) =>  m (List m Bool)
+exSharePutPos =
+  share (share (cons coin nil) >>= \fx -> appM fx fx) >>= \fy -> appM fy fy
+
+exShareListInRepeatedShare :: NDShare (List NDShare Bool)
+exShareListInRepeatedShare =
+  share (share (cons coin nil) >>= \fx -> appM fx fx) >>=
+  \fy -> share coin >>= \fz -> share coin >>= \fa -> cons fz (cons fa fy)
+
+tests = do
+  let exBs  = [ (example1,"ex1",[True,False])
+              , (example2,"ex2",[True,False,True,False])
+              , (example3,"ex3",[True,False,True,False])
+              , (exOr0,"exOr0",[True,False])
+              , (exOr1,"exOr1",[True,True,False])
+              , (exOr2,"exOr2",[True,False])
+              , (exOr2a,"exOr2a",[True,False])
+              , (exOr2b,"exOr2b",[True])
+              , (exOr3,"exOr3",[True,True,True,True])
+              , (exOr3a,"exOr3a",[True,True,False,True,True,False])
+              , (exOr3b,"exOr3b",[True,True,False,True,False])
+              , (exOr3c,"exOr3c",[True,True,False,True,False,True,True,False,True,False])
+              , (exOr4,"exOr4",[True,True,False])
+              , (exOrShare,"exOrShare",[True,True,False])
+              , (exOr6,"exOr6",[True,True,False])
+              , (exOr7,"exOr7",[True,True,False])
+              , (exOr7a,"exOr7a",[True])
+              , (exOr7b,"exOr7b",[True,False])
+              , (exShareConst,"exShareConst",[True,False])
+              , (exShareConstOrR,"exShareConstOrR",[True,False])
+              , (exShareConstOrL,"exShareConstOrL",[True,False])
+              , (exShareConstOrR2,"exShareConstOrR2",[True])
+              , (exFailed,"exFailed",[True])
+              , (exHead,"exHead", [ True, False ])
+              , (exOrShareShare,"exOrShareShare", [True,True,False])
+              , (exOrShareNested,"exOrShareNested", [True,True,False])
+              , (exShareNestedChoiceOr, "exShareNestedChoiceOr", [True,False,True,False])
+              , (exShareIgnoreShare, "exShareIgnoreShare", [True])
+              , (exRepeatedShare, "exRepeatedShare", [True,False])
+              ]
+      exPBs = [ (exDup,"exDup",[ Pair (Identity True) (Identity True)
+                               , Pair (Identity True) (Identity False)
+                               , Pair (Identity False) (Identity True)
+                               , Pair (Identity False) (Identity False)
+                               ])
+              , (exDupShare,"exDupShare",[ Pair (Identity True) (Identity True)
+                                         , Pair (Identity False) (Identity False)
+                                         ])
+              , (exDupShare2,"exDupShare2",[ Pair (Identity True) (Identity True)
+                                           , Pair (Identity False) (Identity False)
+                                           ])
+              , (exDupFailed,"exDupFailed",[ Pair (Identity True) (Identity True) ])
+              , (exDupFirst,"exDupFirst",[ Pair (Identity True) (Identity True)
+                                         , Pair (Identity True) (Identity False)
+                                         , Pair (Identity False) (Identity True)
+                                         , Pair (Identity False) (Identity False)
+                                         ])
+              , (exDupShareFirst,"exShareDupFirst", [ Pair (Identity True) (Identity True)
+                                                    , Pair (Identity False) (Identity False)
+                                                    ])
+              , (exDupShare2,"exDupShare2",[ Pair (Identity True) (Identity True)
+                                           , Pair (Identity False) (Identity False)
+                                           ])
+              , (exShareNestedChoice, "exShareNestedChoice",
+                               [ Pair (Identity True) (Identity True)
+                               , Pair (Identity False) (Identity False)
+                               , Pair (Identity True) (Identity True)
+                               , Pair (Identity False) (Identity False)
+                               ])
+              ]
+      exLBs = [ (exDupl,"exDupl", [ Cons (Identity True) (cons (Identity True) nil)
+                                    , Cons (Identity True) (cons (Identity False) nil)
+                                    , Cons (Identity False) (cons (Identity True) nil)
+                                    , Cons (Identity False) (cons (Identity False) nil)
+                                    ])
+              , (exDuplShare,"exDuplShare", [ Cons (Identity True) (cons (Identity True) nil)
+                                            , Cons (Identity False) (cons (Identity False) nil)
+                                            ])
+              , (exDupl2,"exDupl2", [ Cons (Identity True) (cons (Identity True) nil)
+                                    , Cons (Identity True) (cons (Identity False) nil)
+                                    , Cons (Identity False) (cons (Identity True) nil)
+                                    , Cons (Identity False) (cons (Identity False) nil)
+                                    ])
+              , (exShareNestedChoice2, "exShareNestedChoice2",
+                  [ Cons (Identity True) (cons (Identity True) (cons (Identity True) (cons (Identity True) nil)))
+                  , Cons (Identity True) (cons (Identity False) (cons (Identity True) (cons (Identity False) nil)))
+                  , Cons (Identity False) (cons (Identity True) (cons (Identity False) (cons (Identity True) nil)))
+                  , Cons (Identity False) (cons (Identity False) (cons (Identity False) (cons (Identity False) nil)))
+                  , Cons (Identity True) (cons (Identity True) (cons (Identity True) (cons (Identity True) nil)))
+                  , Cons (Identity True) (cons (Identity False) (cons (Identity True) (cons (Identity False) nil)))
+                  ])
+              , (exOrShareNestedList, "exOrShareNestedList",
+                 [ Cons (Identity True) (cons (Identity True) (cons (Identity True) (cons (Identity True) nil)))
+                 , Cons (Identity True) (cons (Identity False) (cons (Identity True) (cons (Identity False) nil)))
+                 , Cons (Identity False) (cons (Identity True) (cons (Identity False) (cons (Identity True) nil)))
+                 , Cons (Identity False) (cons (Identity False) (cons (Identity False) (cons (Identity False) nil)))
+                 ])
+              ]
+      exLPBs = [ (exShareSingleton, "exShareSingleton", [ Pair (Identity (Cons (Identity True) nil))
+                                                               (Identity (Cons (Identity True) nil))
+                                                        , Pair (Identity (Cons (Identity False) nil))
+                                                               (Identity (Cons (Identity False) nil))
+                                                        ])
+               , (exRecList, "exRecList", [ Pair (cons (Identity True) (cons (Identity False) nil))
+                                                (cons (Identity True) (cons (Identity False) nil))
+                                          , Pair (cons (Identity True) (cons (Identity False) nil))
+                                                 (cons (Identity True) (cons (Identity False) nil))
+                                          , Pair (cons (Identity True) (cons (Identity False) nil))
+                                                (cons (Identity True) (cons (Identity False) nil))
+                                          ])
+               ]
+      maxName = maximum (map (\(_,name,_) -> length name) exBs ++
+                         map (\(_,name,_) -> length name) exPBs ++
+                         map (\(_,name,_) -> length name) exLBs)
+      prettyName name = name ++ ": " ++ replicate (maxName - length name) ' '
+
+  -- Based on the imported implementation, the annotations for `e` might have to be adapted!
+  mapM_ (\(e,name,v) -> putStr (prettyName name) >> pprint (collectVals (e :: NDShare Bool) == v)) exBs
+  mapM_ (\(e,name,v) -> putStr (prettyName name) >> pprint (collectVals (e :: NDShare (Pair NDShare Bool)) == v)) exPBs
+  mapM_ (\(e,name,v) -> putStr (prettyName name) >> pprint (collectVals (e :: NDShare (List NDShare Bool)) == v)) exLBs
+  mapM_ (\(e,name,v) -> putStr (prettyName name) >>
+    pprint (collectVals (e :: NDShare (Pair NDShare (List NDShare Bool))) == v)) exLPBs
+
+*)
